(Re)defined consistency

commute.v
@@ -1,17 +1,22 @@
 Require Import Bool List Streams Logic.Epsilon.
 Import List Notations.
 From Casper 
-Require Import preamble ListExtras ListSetExtras RealsExtras protocol common definitions vlsm indexed_vlsm.
+Require Import preamble ListExtras ListSetExtras RealsExtras protocol common definitions vlsm indexed_vlsm indexed_vlsm_projections.
 
 (* 3.1 Decisions on consensus values *) 
 
 (* Need to add consensus values (and decision functions) to VLSM definitions? *) 
-Class VLSM_plus `{VLSM} :=
+Class consensus_values :=
   { C : Type;
     about_C : exists (c1 c2 : C), c1 <> c2;
   }.
 
-Definition decision `{VLSM_plus} : Type := state -> option C -> Prop. 
+
+(** TODO: Define projection friendliness **)
+(** TODO: Make function **)
+
+Definition decision {message} (S : LSM_sig message) {CV : consensus_values} : Type
+  := @state _ S -> option C -> Prop. 
 
 (* 3.2.1 Decision finality *)
 (* Program Definition prot_state0 `{VLSM} : protocol_state := 
@@ -22,8 +27,9 @@ Next Obligation.
   constructor.
 Defined. *)
 
-Definition final `{VLSM_plus} : decision -> Prop :=
-  fun (D : decision) => forall (tr : protocol_trace), 
+Definition final {message} {S : LSM_sig message} (V : @VLSM message S) {CV : consensus_values}
+  : decision S -> Prop :=
+  fun (D : decision S) => forall (tr : protocol_trace), 
       forall (n1 n2 : nat) (s1 s2 : state) (c1 c2 : C),
         (trace_nth (proj1_sig tr) n1 = Some s1) ->
         (trace_nth (proj1_sig tr) n2 = Some s2) ->
@@ -36,23 +42,130 @@ Definition in_trace `{VLSM} : state -> Trace -> Prop :=
   fun (s : state) (tr : Trace) => exists (n : nat), trace_nth tr n = Some s.
 
 Definition consistent
-  {index : Set}
-  {message : Type}
-  `{VLSM_plus}
-  (IS : index -> LSM_sig message)
-  (IM : forall i : index, @VLSM message (IS i))
-  (ID : index -> decision)
+  {CV : consensus_values}
+  {index : Set} `{Heqd : EqDec index}
+  {message : Type} 
+  {IS : index -> LSM_sig message}
+  {IM : forall i : index, @VLSM message (IS i)}
+  {Hi : index}
+  (constraint : indexed_label IS -> indexed_state IS * option (indexed_proto_message IS) -> Prop)
+  (X := indexed_vlsm_constrained IM Hi constraint)
+  (ID : forall i : index, decision (IS i))
   : Prop
   :=
     (* Assuming we want traces of the overall protocol *)
-    forall (tr : protocol_trace) (s : state),
+    forall (tr : @protocol_trace _ _ X) (s : @state _ (sign X)), True.
+
+(**
       in_trace s (proj1_sig tr) ->
       forall (n1 n2 j k : index),
       exists (c1 c2 : C),
         (ID n1) s (Some c1) -> (ID n2) s (Some c2) ->
         forall (c : C),
-          (ID n1) s (Some c) <-> (ID n2) s (Some c).       
-  
+          (ID n1) s (Some c) <-> (ID n2) s (Some c).    
+**)
+
+Definition consistent_mihai
+  {CV : consensus_values}
+  {index : Set} `{Heqd : EqDec index}
+  {message : Type} 
+  {IS : index -> LSM_sig message}
+  (IM : forall i : index, @VLSM message (IS i))
+  (Hi : index)
+  (constraint : indexed_label IS -> indexed_state IS * option (indexed_proto_message IS) -> Prop)
+  (X := indexed_vlsm_constrained IM Hi constraint)
+  (ID : forall i : index, decision (IS i)) : Prop
+  :=
+    forall (tr : @protocol_trace _ _ X), 
+    forall (n1 n2 : nat),
+    forall (j k : index),
+    forall (s1 s2 : @state _ (sign X)),
+    forall (c1 c2 : C),
+    j <> k ->
+    trace_nth (proj1_sig tr) n1 = (Some s1) ->
+    trace_nth (proj1_sig tr) n2 = (Some s2) ->
+    (ID j) (@s1 j) (Some c1) -> 
+    (ID k) (@s2 k) (Some c2) -> 
+    c1 = c2.
+
+(**Like consistent_mihai, but no longer requiring j <> k, which should imply finality in projections**)
+
+Definition final_and_consistent_mihai
+  {CV : consensus_values}
+  {index : Set} `{Heqd : EqDec index}
+  {message : Type} 
+  {IS : index -> LSM_sig message}
+  (IM : forall i : index, @VLSM message (IS i))
+  (Hi : index)
+  (constraint : indexed_label IS -> indexed_state IS * option (indexed_proto_message IS) -> Prop)
+  (X := indexed_vlsm_constrained IM Hi constraint)
+  (ID : forall i : index, decision (IS i)) : Prop
+  :=
+    forall (tr : @protocol_trace _ _ X), 
+    forall (n1 n2 : nat),
+    forall (j k : index),
+    forall (s1 s2 : @state _ (sign X)),
+    forall (c1 c2 : C),
+    trace_nth (proj1_sig tr) n1 = (Some s1) ->
+    trace_nth (proj1_sig tr) n2 = (Some s2) ->
+    (ID j) (@s1 j) (Some c1) -> 
+    (ID k) (@s2 k) (Some c2) -> 
+    c1 = c2.
+
+Check final_and_consistent_mihai.
+
+Lemma final_and_consistent_implies_consistent 
+  {CV : consensus_values}
+  {index : Set} `{Heqd : EqDec index}
+  {message : Type} 
+  {IS : index -> LSM_sig message}
+  (IM : forall i : index, @VLSM message (IS i))
+  (Hi : index)
+  (constraint : indexed_label IS -> indexed_state IS * option (indexed_proto_message IS) -> Prop)
+  (X := indexed_vlsm_constrained IM Hi constraint)
+  (ID : forall i : index, decision (IS i))
+  : 
+    final_and_consistent_mihai IM Hi constraint ID ->
+    consistent_mihai IM Hi constraint ID.
+
+Proof.
+   intros.
+   unfold final_and_consistent_mihai in H.
+   unfold consistent_mihai.
+   intros.
+   apply H with (tr := tr )(j := j) (n1 := n1) (n2 := n2) (k := k) (s1 := s1) (s2 := s2).
+   - apply H1.
+   - apply H2.
+   - apply H3.
+   - apply H4.
+Qed.
+
+Check final.
+
+Lemma final_and_consistent_implies_final
+  {CV : consensus_values}
+  {index : Set} `{Heqd : EqDec index}
+  {message : Type} 
+  {IS : index -> LSM_sig message}
+  (IM : forall i : index, @VLSM message (IS i))
+  (Hi : index)
+  (constraint : indexed_label IS -> indexed_state IS * option (indexed_proto_message IS) -> Prop)
+  (X := indexed_vlsm_constrained IM Hi constraint)
+  (ID : forall i : index, decision (IS i))
+  : 
+    final_and_consistent_mihai IM Hi constraint ID ->
+    forall i : index, final (indexed_vlsm_constrained_projection IM Hi constraint i) (ID i).
+
+Proof.
+  unfold final_and_consistent_mihai.
+  intros.
+  unfold final.
+  intros.
+  Admitted.
+Qed.
+
+
+
 (* 3.3.1 Initial protocol state bivalence *)
 Definition bivalent `{VLSM_plus} : decision -> Prop :=
   fun (D : decision) =>
